

Part B

Tolkym bai Bekarys

$$x = \begin{bmatrix} 20 \\ 3 \\ 4 \end{bmatrix}$$

$$g = 18$$

$$b_2 = [0,5]$$

$$w_1 = \begin{bmatrix} 0,1 & 0,2 & 0,3 \\ 0,4 & 0,5 & 0,6 \\ 0,7 & 0,8 & 0,9 \end{bmatrix}$$

$$b_1 = \begin{bmatrix} 0,1 \\ 0,2 \\ 0,3 \end{bmatrix}$$

$$w_2 = [0,2; 0,4; 0,6]$$

Forward propagation

$$\textcircled{1} z_1 = w_1 \cdot x + b_1$$

$$z_1 = \begin{bmatrix} 0,1 & 0,2 & 0,3 \\ 0,4 & 0,5 & 0,6 \\ 0,7 & 0,8 & 0,9 \end{bmatrix} \cdot \begin{bmatrix} 20 \\ 3 \\ 4 \end{bmatrix} + \begin{bmatrix} 0,1 \\ 0,2 \\ 0,3 \end{bmatrix}$$

$$R_1 = ((0,1 \cdot 20) + (0,2 \cdot 3) + (0,3 \cdot 4)) + 0,1 = 3,9$$

$$R_2 = ((0,4 \cdot 20) + (0,5 \cdot 3) + (0,6 \cdot 4)) + 0,2 = 12,1$$

$$R_3 = ((0,7 \cdot 20) + (0,8 \cdot 3) + (0,9 \cdot 4)) + 0,3 = 20,3$$

$$z_1 = \begin{bmatrix} 3,9 \\ 12,1 \\ 20,3 \end{bmatrix}$$

$$\textcircled{2} A_1 = \text{ReLU}(z_1)$$

$$A_1 = [3,9; 12,1; 20,3]$$

$$\textcircled{3} z_2 = w_2^T A_1 + b_2 = 18,3$$

$$\textcircled{4} A_2 = a(z_2) = \frac{1}{1 + e^{-1.83}} \approx 1$$

$$\textcircled{5} \text{ Calculate loss: } (A_2 - g)^2$$

$$\text{Loss} = (1 - 1.8)^2 = 2.89$$

Backward propagation

$$\textcircled{1} \frac{dL}{dA_2} = 2 \cdot (1 - 1.8) \approx -3.4$$

$$\textcircled{2} \frac{dL}{dz_2} = -3.74 \cdot 10^{-7}$$

$$\textcircled{3} \frac{dL}{dw_2} = [-1.46 \cdot 10^{-6}, -4.53 \cdot 10^{-6}, -7.59 \cdot 10^{-7}]$$

$$\textcircled{4} \frac{dL}{db_2} = -3.74 \cdot 10^{-7}$$

$$\textcircled{5} \frac{dL}{dA_1} = [-7.48 \cdot 10^{-8}, 1.50 \cdot 10^{-7}, -2.24 \cdot 10^{-7}]$$

$$\textcircled{6} \frac{dL}{dw_1} = \begin{bmatrix} -1.50 \cdot 10^{-6} & -2.24 \cdot 10^{-7} & -2.99 \cdot 10^{-7} \\ -3.00 \cdot 10^{-6} & -4.50 \cdot 10^{-7} & -6.00 \cdot 10^{-7} \\ -4.48 \cdot 10^{-6} & -6.72 \cdot 10^{-7} & -8.97 \cdot 10^{-7} \end{bmatrix}$$

$$\textcircled{7} \frac{dL}{dz_1} = [-7.48 \cdot 10^{-8}, -1.5 \cdot 10^{-7}, -2.24 \cdot 10^{-7}]$$

$$x = 1$$

$$(f - g)^2$$

from

4

$$f(x) = 10^{-6} - 159 \ln$$

$$\textcircled{a} \frac{df}{dx} = 1 - 1.59 \ln^{-1} - 159 \ln^{-2}$$

$$1 = 1.59$$

$$\frac{df}{dx} = 1 - 1.59 \ln^{-1} - 159 \ln^{-2}$$

$$\frac{df}{dx} = 1 - 1.59 \ln^{-1}$$

$$\frac{df}{dx} = 1 - 1.59 \ln^{-1}$$

$\ln(1.59)$